manually apply monotonicity invariants to client server

messageInvariantPrototypes/clientServer/decentralizedMonotonic_globalHistory/applicationProof.dfy
@@ -1,9 +1,11 @@
+include "monotonicityInvariants.dfy"
 include "messageInvariants.dfy"
 
 module ClientServerProof {
 import opened Types
 import opened UtilitiesLibrary
 import opened DistributedSystem
+import opened MonotonicityInvariants
 import opened MessageInvariants
 import opened Obligations
 
@@ -11,25 +13,6 @@ import opened Obligations
 /***************************************************************************************
 *                                Application Invariants                                *
 ***************************************************************************************/
-
-ghost predicate ClientRequestsMonotonic(c: Constants, v: Variables)
-  requires v.WF(c)
-{
-  forall i, j, idx:nat |
-    && v.ValidHistoryIdx(i)
-    && v.ValidHistoryIdx(j)
-    && i <= j
-    && c.ValidClientIdx(idx) 
-  :: 
-    && v.History(i).clients[idx].requests <= 
-        v.History(j).clients[idx].requests
-}
-
-ghost predicate MonotonicityInv(c: Constants, v: Variables)
-  requires v.WF(c)
-{
-  ClientRequestsMonotonic(c, v)
-}
 
 
 // The server's requests must have come from sender client
@@ -42,7 +25,7 @@ ghost predicate ServerRequestsValid(c: Constants, v: Variables)
   ::
     && var req := v.History(i).GetServer(c).currentRequest.value;
     && c.ValidClientIdx(req.clientId)
-    && req.reqId in v.History(i).clients[req.clientId].requests
+    && req.reqId in v.History(i).clients[req.clientId].requests.s
 }
 
 ghost predicate ApplicationInv(c: Constants, v: Variables)
@@ -69,6 +52,7 @@ lemma InitImpliesInv(c: Constants, v: Variables)
   requires Init(c, v)
   ensures Inv(c, v)
 {
+  InitImpliesMonotonicityInv(c, v);
   InitImpliesMessageInv(c, v);
 }
 
@@ -78,23 +62,14 @@ lemma InvInductive(c: Constants, v: Variables, v': Variables)
   ensures Inv(c, v')
 {
   VariableNextProperties(c, v, v');
+  MonotonicityInvInductive(c, v, v');
   MessageInvInductive(c, v, v');
-  InvNextClientRequestsMonotonic(c, v, v');
   InvNextServerRequestsValid(c, v, v');
 }
 
 /***************************************************************************************
 *                                        Proof                                         *
 ***************************************************************************************/
-
-lemma InvNextClientRequestsMonotonic(c: Constants, v: Variables, v': Variables)
-  requires v.WF(c)
-  requires ClientRequestsMonotonic(c, v)
-  requires Next(c, v, v')
-  ensures ClientRequestsMonotonic(c, v')
-{
-  VariableNextProperties(c, v, v');
-}
 
 lemma InvNextServerRequestsValid(c: Constants, v: Variables, v': Variables)
   requires Inv(c, v)
@@ -108,7 +83,7 @@ lemma InvNextServerRequestsValid(c: Constants, v: Variables, v': Variables)
   ensures
     && var req := v'.History(i).GetServer(c).currentRequest.value;
     && c.ValidClientIdx(req.clientId)
-    && req.reqId in v'.History(i).clients[req.clientId].requests
+    && req.reqId in v'.History(i).clients[req.clientId].requests.s
   {}
 }
 
