messageInvariantPrototypes/clientServer/decentralizedMonotonic_globalHistory/monotonicityInvariants.dfy
@@ -1,0 +1,47 @@
+include "spec.dfy"
+
+module MonotonicityInvariants {
+import opened Types
+import opened UtilitiesLibrary
+import opened MonotonicityLibrary
+import opened DistributedSystem
+
+/***************************************************************************************
+*                               Monotonicity Invariants                                *
+***************************************************************************************/
+
+ghost predicate ClientRequestsMonotonic(c: Constants, v: Variables)
+  requires v.WF(c)
+{
+  forall i, j, idx:nat |
+    && v.ValidHistoryIdx(i)
+    && v.ValidHistoryIdx(j)
+    && i <= j
+    && c.ValidClientIdx(idx) 
+  :: 
+    v.History(j).clients[idx].requests.SatisfiesMonotonic(v.History(i).clients[idx].requests)
+}
+
+ghost predicate MonotonicityInv(c: Constants, v: Variables) 
+{
+  && v.WF(c)
+  && ClientRequestsMonotonic(c, v)
+}
+
+// Base obligation
+lemma InitImpliesMonotonicityInv(c: Constants, v: Variables)
+  requires Init(c, v)
+  ensures MonotonicityInv(c, v)
+{}
+
+// Inductive obligation
+lemma MonotonicityInvInductive(c: Constants, v: Variables, v': Variables)
+  requires MonotonicityInv(c, v)
+  requires Next(c, v, v')
+  ensures MonotonicityInv(c, v')
+{
+  VariableNextProperties(c, v, v');
+}
+
+} // end module MonotonicityInvariants
+
