messageInvariantPrototypes/clientServer/types.dfy
@@ -1,4 +1,4 @@
-include "../lib/UtilitiesLibrary.dfy"
+include "../lib/MonotonicityLibrary.dfy"
 
 module Types {
   import opened UtilitiesLibrary
